src/Polara/Codegeneration/Python/Codegeneration.lean
@@ -24,6 +24,7 @@ def Const2.tmgenPy (a: String) (b: String): Const2 α₁ α₂ α → String
   | lt => s!"{a} < {b}"
   | maxf => s!"max({a}, {b})"
   | addi => s!"{a} + {b}"
+  | eqi  => s!"{a} == {b}"
   | tup  => s!"({a}, {b})"
   | app  => s!"{a}({b})"
   | get  => s!"{a}[{b}]"
