src/Polara/Optimizations/Defunc.lean
@@ -1,0 +1,83 @@
+import Polara.Syntax.Index
+
+-- but everything as function from an env?
+-- ainf?
+
+@[reducible]
+def Ty.defunc: Ty → Ty :=
+  Ty.map (λ
+  | _ ~> _ => .unit
+  | α => α)
+
+-- @[reducible]
+-- def Ty.defuncMeta: Ty → Type :=
+
+
+#eval (.flt ×× .flt).defunc
+#eval (.flt ~> .flt).defunc
+#eval (.flt ×× (.flt ~> .flt)).defunc
+#eval (.flt ~> (.flt ~> .flt)).defunc
+
+def Const0.defunc: Const0 α → Tm Γ α.defunc
+| .litl l => tlitl l
+| .litn n => tlitn n
+| .litf f => tlitf f
+| .liti i => tliti i
+| .litu => tlitu
+| .mkRef => Tm.mkRef
+
+def Const1.defunc (x: Tm Γ α.defunc): Const1 α β → Tm Γ β.defunc
+| .suml     => Tm.cst1 Const1.suml x
+| .exp      => Tm.cst1 Const1.exp x
+| .sqrt     => Tm.cst1 Const1.sqrt x
+| .log      => Tm.cst1 Const1.log x
+| .normCdf  => Tm.cst1 Const1.normCdf x
+| .fst      => Tm.cst1 Const1.fst x
+| .snd      => Tm.cst1 Const1.snd x
+| .sumf     => Tm.cst1 Const1.sumf x
+| .i2n      => Tm.cst1 Const1.i2n x
+| .n2f      => Tm.cst1 Const1.n2f x
+| .refGet   => Tm.cst1 Const1.refGet x
+
+def Const2.defunc (a: Tm Γ α.defunc)(b: Tm Γ β.defunc): Const2 α β γ → Tm Γ γ.defunc
+| linOp (type:=t) op =>
+  have: BiArraysC BiLin α.defunc β.defunc γ.defunc := ⟨
+    let rec goO {α β γ: Ty}: BiArrays BiLin α β γ → BiArrays BiLin α.defunc β.defunc γ.defunc
+    | .array n t' => .array n (goO t')
+    | .base t' => .base (match t' with | .lins => .lins)
+    goO t.t⟩
+  Tm.cst2 (.linOp op) a b
+| linScale (type:=t) op =>
+  have: BiArrayC BiLF α.defunc β.defunc γ.defunc := ⟨
+    let goS {α β γ: Ty}: BiLF α β γ → BiLF α.defunc β.defunc γ.defunc := λ | .lf => .lf
+    match t.t with
+    | .array n t' => .array n (goS t')
+    | .base t' => .base (goS t')
+  ⟩
+  Tm.cst2 (.linScale op) a b
+| .arithOp (type:=t) op =>
+  have: BiArraysC BiArith α.defunc β.defunc γ.defunc := ⟨
+    let rec goA {α β γ: Ty}: BiArrays BiArith α β γ → BiArrays BiArith α.defunc β.defunc γ.defunc
+    | .array n t' => .array n (goA t')
+    | .base t' => .base (match t' with | .nats => .nats | .flts => .flts)
+    goA t.t⟩
+  Tm.cst2 (.arithOp op) a b
+| .addi   => Tm.cst2 .addi a b
+| .maxf   => Tm.cst2 maxf a b
+| .lt     => Tm.cst2 .lt a b
+| .eqi    => Tm.cst2 .eqi a b
+| .get    => Tm.cst2 .get a b
+| .tup    => Tm.cst2 .tup a b
+| .refSet => Tm.cst2 .refSet a b
+| .app  => sorry -- complete
+
+def Tm.defunc : Tm VPar α → Tm VPar α.defunc
+| .err => .err
+| .cst0 const0 => const0.defunc
+| .cst1 const1 t => const1.defunc t.defunc
+| .cst2 const2 a b => const2.defunc a.defunc b.defunc
+| .abs f => ()'
+| .bld a => .bld (λ idx => (a idx).defunc)
+| .ite cond a b => .ite cond.defunc a.defunc b.defunc
+| .var v => .var v.changeType
+| .bnd rest l => .bnd rest.defunc (λ v => (l v.changeType).defunc)
