src/Polara/Optimizations/Vectorization.lean
@@ -1,6 +1,23 @@
 import Polara.Optimizations.Basics
 import Polara.Optimizations.CleanEnv
 
+private def vectorize' [t : BiArraysC BiArith α β γ](envPre envC envA envB: Env)(v: Var γ)(a: VPar α)(b: VPar β)(op: ArithOp): VParM Bnds :=
+  match envPre with -- todo allow multiple forc
+  | (.forc n i) :: env' => do
+    let ar := (←VParM.var) (α.array n)
+    let br := (←VParM.var) (β.array n)
+    let cr := (←VParM.var) (γ.array n)
+    return [
+      -- env in val
+      ⟨⟨_,ar⟩, (env'.append envA), Prim.bld i a⟩,
+      ⟨⟨_,br⟩, (env'.append envB), Prim.bld i b⟩,
+      -- vec op
+      ⟨⟨_,cr⟩, (env'.append envC), Prim.cst2 (.arithOp op) (.v ar) (.v br)⟩,
+      -- val in vec
+      ⟨⟨_,v ⟩, (envPre.append envC) , Prim.cst2 (.get) (.v cr) (.p i)⟩
+    ]
+  | _ => pure [⟨⟨_,v⟩, (envPre.append envC), Prim.cst2 (.arithOp op) a b⟩]
+
 def AINF.vectorize (ainf: AINF α): AINF α :=
   ainf.flatMapMBnd id (λ bnd => match bnd with
     | ⟨⟨α,v⟩,env,prim⟩ =>
@@ -18,6 +35,7 @@ def AINF.vectorize (ainf: AINF α): AINF α :=
           let bER := restPrefixes[2]
           match cst2 with
           | .arithOp (type:=_) op =>
+            -- vectorize' env
             match envPrefix with -- todo allow multiple forc
             | (.forc n i) :: env' => do
               let ar := (←VParM.var) (α'.array n)
@@ -41,6 +59,7 @@ def AINF.vectorize (ainf: AINF α): AINF α :=
 open Ty
 #eval (for' i:10 => tlitf 1 + tlitf 1).toAINF.cleanEnv.vectorize -- no vecotrization
 #eval (fun' a => for' i:10 => a[[i]] + (tlitf 1)).toAINF.cleanEnv.vectorize -- no vectorize?
+
 #eval (fun' a: flt.array 10 => for' i:10 => a[[i]] + a[[i]]).toAINF.cleanEnv.vectorize -- vectorize
 #eval (fun' a => for' i:10 => (a[[i]] + a[[i]]) + a[[i]]).toAINF.cleanEnv.vectorize -- vectorize
 
